Refinement/soundness on arbitrary number of reductions Composition of configurations preserve run semantics Strange behavior of `auto` when trying proof of completeness

Operational.thy
@@ -7,13 +7,11 @@ begin
 text{* Operational steps *}
 
 abbreviation uncurry_conf
-  :: "system \<Rightarrow> instant_index \<Rightarrow> TESL_formula \<Rightarrow> TESL_formula
-   \<Rightarrow> (system \<times> instant_index \<times> TESL_formula \<times> TESL_formula)" ("_, _ \<turnstile> _ \<triangleright> _" 50) where
+  :: "system \<Rightarrow> instant_index \<Rightarrow> TESL_formula \<Rightarrow> TESL_formula \<Rightarrow> config" ("_, _ \<turnstile> _ \<triangleright> _" 50) where
   "\<Gamma>, n \<turnstile> \<Psi> \<triangleright> \<Phi> \<equiv> (\<Gamma>, n, \<Psi>, \<Phi>)"
 
 inductive operational_semantics_step
-  :: "(system \<times> instant_index \<times> TESL_formula \<times> TESL_formula)
-    \<Rightarrow> (system \<times> instant_index \<times> TESL_formula \<times> TESL_formula) \<Rightarrow> bool" ("_ \<hookrightarrow> _" 50) where
+  :: "config \<Rightarrow> config \<Rightarrow> bool" ("_ \<hookrightarrow> _" 50) where
   instant_i:
   "consistent_run \<Gamma> \<Longrightarrow>
    \<Gamma>, n \<turnstile> [] \<triangleright> \<Phi>
@@ -55,14 +53,29 @@ inductive operational_semantics_step
    \<Gamma>, n \<turnstile> (K\<^sub>1 time-delayed by \<delta>\<tau> on K\<^sub>2 implies K\<^sub>3) # \<Psi> \<triangleright> \<Phi>
      \<hookrightarrow>  K\<^sub>1 \<Up> n # \<Gamma>, n \<turnstile> (K\<^sub>3 sporadic \<lfloor>\<tau>\<^sub>v\<^sub>a\<^sub>r(K\<^sub>2, n) \<oplus> \<delta>\<tau>\<rfloor> on K\<^sub>2) # \<Psi> \<triangleright> (K\<^sub>1 time-delayed by \<delta>\<tau> on K\<^sub>2 implies K\<^sub>3) # \<Phi>"
 
-abbreviation operational_semantics_step'
-  :: "(system \<times> instant_index \<times> TESL_formula \<times> TESL_formula) rel" ("\<hookrightarrow>\<^sup>\<up>") where
+abbreviation operational_semantics_rellifted
+  :: "config rel" ("\<hookrightarrow>\<^sup>\<up>") where
   "\<hookrightarrow>\<^sup>\<up> \<equiv> { ((\<Gamma>\<^sub>1, n\<^sub>1, \<Psi>\<^sub>1, \<Phi>\<^sub>1), (\<Gamma>\<^sub>2, n\<^sub>2, \<Psi>\<^sub>2, \<Phi>\<^sub>2)).
               \<Gamma>\<^sub>1, n\<^sub>1 \<turnstile> \<Psi>\<^sub>1 \<triangleright> \<Phi>\<^sub>1 \<hookrightarrow> \<Gamma>\<^sub>2, n\<^sub>2 \<turnstile> \<Psi>\<^sub>2 \<triangleright> \<Phi>\<^sub>2 }"
 
+lemma rel_uncurry_equiv:
+  shows "(\<S>\<^sub>1, \<S>\<^sub>2) \<in> \<hookrightarrow>\<^sup>\<up> \<longleftrightarrow> \<S>\<^sub>1 \<hookrightarrow> \<S>\<^sub>2"
+  by auto
+
+abbreviation operational_semantics_rellifted_elim
+  :: "config rel" ("\<hookrightarrow>\<^sub>e") where
+  "\<hookrightarrow>\<^sub>e \<equiv> { ((\<Gamma>\<^sub>1, n, \<Psi>\<^sub>1, \<Phi>\<^sub>1), (\<Gamma>\<^sub>2, n, \<Psi>\<^sub>2, \<Phi>\<^sub>2)).
+              \<Gamma>\<^sub>1, n \<turnstile> \<Psi>\<^sub>1 \<triangleright> \<Phi>\<^sub>1 \<hookrightarrow> \<Gamma>\<^sub>2, n \<turnstile> \<Psi>\<^sub>2 \<triangleright> \<Phi>\<^sub>2 }"
+
+abbreviation operational_semantics_rellifted_intro
+  :: "config rel" ("\<hookrightarrow>\<^sub>i") where
+  "\<hookrightarrow>\<^sub>i \<equiv> { ((\<Gamma>\<^sub>1, n\<^sub>1, \<Psi>\<^sub>1, \<Phi>\<^sub>1), (\<Gamma>\<^sub>2, n\<^sub>2, \<Psi>\<^sub>2, \<Phi>\<^sub>2)).
+              n\<^sub>2 = Suc n\<^sub>1
+              \<and> \<Gamma>\<^sub>1, n\<^sub>1 \<turnstile> \<Psi>\<^sub>1 \<triangleright> \<Phi>\<^sub>1 \<hookrightarrow> \<Gamma>\<^sub>2, n\<^sub>2 \<turnstile> \<Psi>\<^sub>2 \<triangleright> \<Phi>\<^sub>2 }"
+
 abbreviation operational_semantics_simulation_step
-  :: "(system \<times> instant_index \<times> TESL_formula \<times> TESL_formula) rel" ("\<hookrightarrow>\<^sup>\<nabla>") where
-  "\<hookrightarrow>\<^sup>\<nabla> \<equiv> { ((\<Gamma>\<^sub>1, n\<^sub>1, \<Psi>, \<Phi>\<^sub>1), (\<Gamma>\<^sub>2, n\<^sub>2, \<Psi>, \<Phi>\<^sub>2)).
+  :: "config rel" ("\<hookrightarrow>\<^sub>\<nabla>") where
+  "\<hookrightarrow>\<^sub>\<nabla> \<equiv> { ((\<Gamma>\<^sub>1, n\<^sub>1, \<Psi>, \<Phi>\<^sub>1), (\<Gamma>\<^sub>2, n\<^sub>2, \<Psi>, \<Phi>\<^sub>2)).
                 \<Psi> = []
               \<and> (\<Gamma>\<^sub>1, n\<^sub>1 \<turnstile> \<Psi> \<triangleright> \<Phi>\<^sub>1, \<Gamma>\<^sub>2, n\<^sub>2 \<turnstile> \<Psi> \<triangleright> \<Phi>\<^sub>2) \<in> \<hookrightarrow>\<^sup>\<up>\<^sup>+
               \<and> consistent_run \<Gamma>\<^sub>1
@@ -72,7 +85,7 @@ abbreviation operational_semantics_simulation_step
 (* Note that \<hookrightarrow>\<^sub>\<nabla> is unfolded as necessary as it is to eliminate \<psi>-formulae *)
 lemma "([], 0        \<turnstile> [] \<triangleright> [H\<^sub>1 sporadic \<tau>\<^sub>i\<^sub>n\<^sub>t 0, H\<^sub>1 implies H\<^sub>2],
          \<Gamma>, 1 \<turnstile> [] \<triangleright> \<Phi>)
-         \<in> \<hookrightarrow>\<^sup>\<nabla>"
+         \<in> \<hookrightarrow>\<^sub>\<nabla>"
 apply auto
 apply (rule trancl_into_trancl)
 apply (rule trancl_into_trancl)
@@ -84,8 +97,7 @@ apply (rule sporadic_e2)
   apply (rule witness_consistency, auto, ((simp add: Abs_run_inverse_rewrite mono_iff_le_Suc)+)?)
 sorry (* OK *)
 
-inductive finite_SAT
-  :: "(system \<times> instant_index \<times> TESL_formula \<times> TESL_formula) \<Rightarrow> bool" ("\<TTurnstile> _" 50) where
+inductive finite_SAT :: "config \<Rightarrow> bool" ("\<TTurnstile> _" 50) where
   finite_SAT_ax: "set (NoSporadic \<Phi>) = set \<Phi> \<Longrightarrow>
                     consistent_run \<Gamma> \<Longrightarrow>
                    \<TTurnstile> \<Gamma>, n \<turnstile> \<Psi> \<triangleright> \<Phi>"
